meta-theory/pure_exp_eq_in_ctxtScript.sml
@@ -1,0 +1,641 @@
+(*
+  Formalize the notion of context and a new relation coming with it
+*)
+
+open HolKernel Parse boolLib bossLib term_tactic;
+open arithmeticTheory listTheory stringTheory alistTheory dep_rewrite
+     optionTheory pairTheory ltreeTheory llistTheory bagTheory
+     BasicProvers pred_setTheory relationTheory rich_listTheory finite_mapTheory;
+open pure_expTheory pure_valueTheory pure_evalTheory pure_eval_lemmasTheory
+     pure_exp_lemmasTheory pure_miscTheory pure_exp_relTheory pure_congruenceTheory;
+open  pure_alpha_equivTheory;
+
+val _ = new_theory "pure_exp_eq_in_ctxt";
+
+(* Preliminaries *)
+
+Theorem exp_eq_l_refl:
+  ∀b l. LIST_REL (λx y. (x ≅? y) b) l l
+Proof
+  gen_tac
+  \\ Induct
+  \\ fs [exp_eq_refl]
+QED
+
+Theorem eval_Prim:
+  ∀ope eL eL'. LIST_REL (λe1 e2. eval e1 = eval e2) eL eL' ⇒ eval (Prim ope eL) = eval (Prim ope eL')
+Proof
+  Cases
+  \\ rw [eval_thm]
+  >~[‘MAP _ _ = MAP _ _’]
+  >- (irule LIST_EQ
+      \\ gvs [LIST_REL_EL_EQN, EL_MAP])
+  >~[‘AtomOp’]
+  >- (fs [eval_def]
+      \\ once_rewrite_tac [v_unfold]
+      \\ fs [eval_wh_Prim]
+      \\ qsuff_tac ‘get_atoms (MAP eval_wh eL') = get_atoms (MAP eval_wh eL)’
+      >- (CASE_TAC \\ fs [])
+      \\ fs [get_atoms_def]
+      \\ qsuff_tac ‘EXISTS error_Atom (MAP eval_wh eL) ⇔ EXISTS error_Atom (MAP eval_wh eL')’
+      >- (strip_tac
+          \\ IF_CASES_TAC
+          \\ simp []
+          \\ qsuff_tac ‘MEM wh_Diverge (MAP eval_wh eL) ⇔ MEM wh_Diverge (MAP eval_wh eL')’
+          >- (strip_tac
+              \\ IF_CASES_TAC
+              \\ simp []
+              \\ irule LIST_EQ
+              \\ rw []
+              \\ gvs [LIST_REL_EL_EQN, EL_MAP, EVERY_EL]
+              \\ rpt $ first_x_assum drule
+              \\ once_rewrite_tac [v_unfold]
+              \\ rpt FULL_CASE_TAC
+              \\ rw [dest_Atom_def, error_Atom_def])
+          \\ eq_tac
+          \\ strip_tac
+          \\ gvs [MEM_EL, LIST_REL_EL_EQN]
+          \\ first_assum $ irule_at Any
+          \\ first_assum drule
+          \\ once_rewrite_tac [v_unfold]
+          \\ rpt FULL_CASE_TAC
+          \\ gvs [EL_MAP])
+      \\ eq_tac
+      \\ strip_tac
+      \\ gvs [EXISTS_MEM, MEM_EL, EL_MAP, LIST_REL_EL_EQN]
+      \\ rename1 ‘MAP eval_wh eL2’
+      \\ qexists_tac ‘eval_wh (EL n eL2)’
+      \\ first_x_assum drule
+      \\ once_rewrite_tac [v_unfold]
+      \\ rpt FULL_CASE_TAC
+      \\ fs [error_Atom_def]
+      \\ rw []
+      \\ first_assum $ irule_at Any
+      \\ fs [EL_MAP])
+  \\ Cases_on ‘eL’ \\ Cases_on ‘eL'’ \\ fs []
+  \\ rename1 ‘LIST_REL _ t1 t2’
+  \\ Cases_on ‘t1’ \\ Cases_on ‘t2’ \\ gvs [eval_thm]
+  >~[‘Prim Seq (_::_::_)’]
+  >- (rename1 ‘LIST_REL _ t1 t2’
+      \\ Cases_on ‘t1’ \\ Cases_on ‘t2’
+      \\ gvs [eval_thm, eval_def]
+      \\ once_rewrite_tac [v_unfold]
+      \\ fs [eval_wh_Prim])
+  >~[‘Prim If (_::_::_)’]
+  >- (rename1 ‘LIST_REL _ t1 t2’
+      \\ Cases_on ‘t1’ \\ Cases_on ‘t2’ \\ gvs []
+      >~[‘_::_::_::_’]
+      >- (rename1 ‘LIST_REL _ t1 t2’
+          \\ Cases_on ‘t1’ \\ Cases_on ‘t2’
+          \\ gvs [eval_thm, eval_def]
+          \\ once_rewrite_tac [v_unfold]
+          \\ rw [eval_wh_Prim])
+      \\ rw [eval_def]
+      \\ once_rewrite_tac [v_unfold]
+      \\ rw [eval_wh_Prim])
+  \\ rw [eval_def]
+  \\ once_rewrite_tac [v_unfold]
+  \\ rw [eval_wh_Prim]
+QED
+
+Theorem FLOOKUP_LUPDATE:
+  ∀l f n v. FLOOKUP (f |++ l) n = SOME v ⇒ MEM (n, v) l ∨ FLOOKUP f n = SOME v
+Proof
+  Induct
+  \\ fs [FUPDATE_LIST_THM]
+  \\ PairCases \\ rw []
+  \\ first_x_assum $ dxrule_then assume_tac
+  \\ gvs [FLOOKUP_UPDATE]
+  \\ FULL_CASE_TAC \\ fs []
+QED
+
+Theorem Letrec_Prim:
+  ∀l ope eL b. (Letrec l (Prim ope eL) ≅? Prim ope (MAP (Letrec l) eL)) b
+Proof
+  rw []
+  \\ irule eval_IMP_exp_eq
+  \\ rw [subst_def, eval_thm, subst_funs_def, bind_def]
+  >- (irule eval_Prim
+      \\ rw [LIST_REL_EL_EQN, EL_MAP, subst_def, eval_thm, subst_funs_def]
+      \\ gvs [bind_def]
+      \\ IF_CASES_TAC \\ fs []
+      \\ first_x_assum dxrule
+      \\ strip_tac
+      \\ fs [])
+  \\ fs [MAP_MAP_o]
+  \\ dxrule_then assume_tac FLOOKUP_LUPDATE
+  \\ gvs [FLOOKUP_EMPTY, MEM_EL, EL_MAP]
+  \\ qsuff_tac ‘F’ \\ fs []
+  \\ first_x_assum irule
+  \\ rename1 ‘EL k l’
+  \\ qabbrev_tac ‘p = EL k l’
+  \\ PairCases_on ‘p’
+  \\ gvs [EVERY_EL, EL_MAP]
+  \\ rw []
+  \\ rename1 ‘EL k2 l’
+  \\ qabbrev_tac ‘p' = EL k2 l’
+  \\ PairCases_on ‘p'’
+  \\ gvs []
+  \\ ‘∀v. v ∈ FRANGE (FDIFF f (set (MAP FST l))) ⇒ closed v’
+    by (rw []
+        \\ first_x_assum irule
+        \\ gvs [FRANGE_FLOOKUP, FLOOKUP_FDIFF]
+        \\ pop_assum $ irule_at Any)
+  \\ gvs [freevars_subst, SUBSET_DEF, IN_DIFF, FDOM_FDIFF]
+  \\ rw [MEM_EL]
+  >>~[‘EL _ (MAP FST _) = EL _ (MAP FST _)’]
+  >- (first_assum $ irule_at Any
+      \\ gvs [EL_MAP]
+      \\ rename1 ‘FST p = FST _’
+      \\ PairCases_on ‘p’
+      \\ fs [])
+  >- (first_assum $ irule_at Any
+      \\ gvs [EL_MAP]
+      \\ rename1 ‘FST p = FST _’
+      \\ PairCases_on ‘p’
+      \\ fs [])
+  \\ first_x_assum $ qspecl_then [‘x’] assume_tac
+  \\ pop_assum kall_tac
+  \\ first_x_assum $ qspecl_then [‘x’] assume_tac
+  \\ gvs [] >>~[‘MEM x (MAP FST l)’]
+  >- (gvs [MEM_EL]
+      \\ first_assum $ irule_at Any
+      \\ fs [EL_MAP]
+      \\ rename1 ‘FST p = FST _’
+      \\ PairCases_on ‘p’ \\ fs [])
+  >- (gvs [MEM_EL]
+      \\ first_assum $ irule_at Any
+      \\ fs [EL_MAP]
+      \\ rename1 ‘FST p = FST _’
+      \\ PairCases_on ‘p’ \\ fs [])
+  \\ first_x_assum $ qspecl_then [‘freevars p'1’] assume_tac
+  \\ gvs [MEM_MAP]
+  \\ pop_assum $ qspecl_then [‘EL k2 l’] assume_tac
+  \\ gvs [EL_MEM]
+QED
+
+Theorem Let_Lam:
+  ∀v w e1 e2 b. closed e1 ∧ v ≠ w ⇒ (Let v e1 (Lam w e2) ≅? Lam w (Let v e1 e2)) b
+Proof
+  rw []
+  \\ irule exp_eq_trans
+  \\ irule_at Any beta_equality
+  \\ gvs [subst1_def]
+  \\ irule exp_eq_Lam_cong
+  \\ irule $ iffLR exp_eq_sym
+  \\ irule beta_equality
+  \\ gvs []
+QED
+
+Theorem Let_Lam_weak:
+  ∀v w e1 e2 b. v ≠ w ⇒ w ∉ freevars e1 ⇒ (Let v e1 (Lam w e2) ≅? Lam w (Let v e1 e2)) b
+Proof
+  rw [exp_eq_def, bind_def] >> IF_CASES_TAC >>
+  gvs [app_bisimilarity_eq, exp_eq_refl] >>
+  rpt (irule_at Any IMP_closed_subst) >>
+  drule_then assume_tac $ GSYM subst_fdomsub >>
+  gvs [subst_def, DOMSUB_COMMUTES] >>
+  irule_at Any Let_Lam >>
+  irule_at Any IMP_closed_subst >>
+  rw [FRANGE_FLOOKUP]
+QED
+
+Theorem FDIFF_DOMSUB:
+  ∀f v s. FDIFF (f \\ s) v = (FDIFF f v) \\ s
+Proof
+  rw [FDIFF_def, fmap_domsub, INTER_COMM]
+QED
+
+Theorem MAP_subst_fdomsub:
+  ∀v l f. EVERY (λe. v ∉ freevars e) (MAP SND l) ⇒
+          MAP (λ(s, e). (s, subst (FDIFF f (set (MAP FST l)) \\ v) e)) l
+          = MAP (λ(s, e). (s, subst (FDIFF f (set (MAP FST l))) e)) l
+Proof
+  rw [EVERY_EL] >> irule LIST_EQ >>
+  rw [EL_MAP] >> first_x_assum $ drule_then assume_tac >>
+  rename1 ‘EL x l’ >> qabbrev_tac ‘p = EL x l’ >> PairCases_on ‘p’ >>
+  gvs [subst_fdomsub, EL_MAP]
+QED
+
+Theorem Letrec_Lam:
+  ∀l w e b. EVERY (λe. freevars e ⊆ set (MAP FST l)) (MAP SND l) ∧ ¬MEM w (MAP FST l)
+          ⇒ (Letrec l (Lam w e) ≅? Lam w (Letrec l e)) b
+Proof
+  rw []
+  \\ irule exp_eq_trans
+  \\ irule_at Any beta_equality_Letrec
+  \\ gvs [subst_funs_eq_subst, subst_def]
+  \\ irule exp_eq_Lam_cong
+  \\ irule $ iffLR exp_eq_sym
+  \\ irule exp_eq_trans
+  \\ irule_at Any beta_equality_Letrec
+  \\ gvs [subst_funs_eq_subst]
+  \\ irule eval_IMP_exp_eq
+  \\ rw []
+  \\ rpt AP_TERM_TAC \\ AP_THM_TAC \\ AP_TERM_TAC
+  \\ irule $ GSYM DOMSUB_NOT_IN_DOM
+  \\ gvs [FDOM_FUPDATE_LIST]
+  \\ strip_tac \\ last_x_assum irule
+  \\ gvs [MEM_EL]
+  \\ first_assum $ irule_at Any
+  \\ gvs [EL_MAP]
+  \\ rename1 ‘FST (_ p)’
+  \\ PairCases_on ‘p’
+  \\ fs []
+QED
+
+Theorem Letrec_Lam_weak:
+  ∀l v e b. EVERY (λe. v ∉ freevars e) (MAP SND l) ∧ ¬ MEM v (MAP FST l)
+            ⇒ (Letrec l (Lam v e) ≅? Lam v (Letrec l e)) b
+Proof
+  rw [exp_eq_def, bind_def] >> IF_CASES_TAC >>
+  gvs [app_bisimilarity_eq, exp_eq_refl] >>
+  rpt $ irule_at Any IMP_closed_subst >>
+  gvs [subst_def, FDIFF_DOMSUB, MAP_subst_fdomsub] >>
+  irule_at Any Letrec_Lam >>
+  gvs [MAP_MAP_o, combinTheory.o_DEF, LAMBDA_PROD, EVERY_EL, EL_MAP] >>
+  rw [FRANGE_FLOOKUP]
+  >- (rename1 ‘EL n l’ >> qabbrev_tac ‘p = EL n l’ >>
+      PairCases_on ‘p’ >>
+      ‘∀v. v ∈ FRANGE (FDIFF f (set (MAP FST l))) ⇒ closed v’
+        by (rw [FRANGE_FLOOKUP, FLOOKUP_FDIFF] >>
+            first_x_assum irule >>
+            pop_assum $ irule_at Any) >>
+      gvs [freevars_subst, SUBSET_DEF, IN_DIFF, FDOM_FDIFF] >>
+      gen_tac >> rename1 ‘MEM x _’ >>
+      last_x_assum $ qspecl_then [‘x’] assume_tac >>
+      last_x_assum $ qspecl_then [‘x’] assume_tac >>
+      rw [] >> gvs []
+      >- (last_x_assum $ qspecl_then [‘freevars p1’] assume_tac >>
+          gvs [MEM_MAP] >> pop_assum $ qspecl_then [‘EL n l’] assume_tac >>
+          gvs [EL_MEM])
+      >- (last_x_assum $ qspecl_then [‘freevars p1’] assume_tac >>
+          gvs [MEM_MAP] >> pop_assum $ qspecl_then [‘EL n l’] assume_tac >>
+          gvs [EL_MEM]) >>
+      gvs [MEM_EL] >>
+      first_assum $ irule_at Any >>
+      rw [EL_MAP] >>
+      rename1 ‘FST p2’ >> PairCases_on ‘p2’ >> fs [])
+  >- (strip_tac >> last_x_assum irule >>
+      gvs [MEM_EL] >> first_assum $ irule_at Any >>
+      gvs [EL_MAP] >> rename1 ‘FST p’ >> PairCases_on ‘p’ >>
+      fs [])
+QED
+
+Theorem Letrec_closed:
+  ∀l e b. closed e ⇒ (Letrec l e ≅? e) b
+Proof
+  rw [exp_eq_def, bind_def] >> IF_CASES_TAC >>
+  gvs [app_bisimilarity_eq, exp_eq_refl] >>
+  irule_at (Pos $ el 2) IMP_closed_subst >>
+  gvs [subst_def, closed_subst, FRANGE_FLOOKUP] >>
+  irule exp_eq_trans >>
+  irule_at Any beta_equality_Letrec >>
+  conj_asm1_tac
+  >- (rw [EVERY_EL, EL_MAP, MAP_MAP_o, combinTheory.o_DEF, LAMBDA_PROD] >>
+      rename1 ‘EL n l’ >> qabbrev_tac ‘p = EL n l’ >> PairCases_on ‘p’ >>
+      ‘∀v. v ∈ FRANGE (FDIFF f (set (MAP FST l))) ⇒ closed v’
+        by (rw [FRANGE_FLOOKUP, FLOOKUP_FDIFF] >>
+            first_x_assum irule >>
+            pop_assum $ irule_at Any) >>
+      gvs [freevars_subst, SUBSET_DEF, IN_DIFF, FDOM_FDIFF] >>
+      gen_tac >> rename1 ‘MEM x _’ >>
+      last_x_assum $ qspecl_then [‘x’] assume_tac >>
+      rw [] >> gvs []
+      >- (first_x_assum $ qspecl_then [‘freevars p1’] assume_tac >>
+          gvs [MEM_MAP] >> pop_assum $ qspecl_then [‘EL n l’] assume_tac >>
+          gvs [EL_MEM]) >>
+      gvs [MEM_EL] >>
+      first_assum $ irule_at Any >> rw [EL_MAP] >>
+      rename1 ‘FST p2’ >> PairCases_on ‘p2’ >> fs []) >>
+  dxrule_then assume_tac subst_funs_eq_subst >>
+  rw [exp_eq_refl]
+QED
+
+Theorem Let_Letrec:
+  ∀s l e1 e2 b. EVERY (λe. s ∉ freevars e) (MAP SND l) ∧ ¬MEM s (MAP FST l) ∧ closed e1
+                ⇒ (Let s e1 (Letrec l e2) ≅? Letrec l (Let s e1 e2)) b
+Proof
+  rw [] >>
+  irule exp_eq_trans >>
+  irule_at (Pos hd) exp_eq_App_cong >>
+  irule_at (Pos hd) $ iffLR exp_eq_sym >>
+  irule_at Any Letrec_Lam_weak >> fs [] >>
+  irule_at Any exp_eq_refl >>
+  irule $ iffLR exp_eq_sym >>
+  irule exp_eq_trans >>
+  irule_at Any Letrec_App >>
+  irule exp_eq_App_cong >>
+  gvs [exp_eq_refl, Letrec_closed]
+QED
+
+Theorem Let_Let:
+  ∀v w e1 e2 e3 b. v ≠ w ∧ v ∉ freevars e2 ∧ w ∉ freevars e1 ⇒
+                   (Let v e1 (Let w e2 e3) ≅? Let w e2 (Let v e1 e3)) b
+Proof
+  rw []
+  \\ irule eval_IMP_exp_eq
+  \\ rw [subst_def]
+  \\ rename1 ‘subst (f \\ _ \\ _)’
+  \\ ‘∀v. v ∈ FRANGE f ⇒ closed v’ by (rw [FRANGE_FLOOKUP])
+  \\ drule $ GSYM subst_fdomsub
+  \\ last_x_assum assume_tac
+  \\ last_x_assum assume_tac
+  \\ drule $ GSYM subst_fdomsub
+  \\ rw [eval_Let, subst_def, bind1_def, IMP_closed_subst, DOMSUB_COMMUTES]
+  \\ AP_TERM_TAC
+  \\ rw [fmap_domsub, COMPL_UNION]
+  \\ irule subst1_subst1
+  \\ gvs [IMP_closed_subst]
+QED
+
+(* Part on context *)
+
+Datatype:
+  ctxt = Nil
+       | IsFree string ctxt
+       | Bind string exp ctxt
+       | RecBind ((string # exp) list) ctxt
+End
+
+Definition exp_eq_in_ctxt_def:
+  exp_eq_in_ctxt Nil = (λe1 e2. e1 ≈ e2) ∧
+  exp_eq_in_ctxt (IsFree s c) e1 e2 = (∀e3. closed e3 ⇒ exp_eq_in_ctxt c (Let s e3 e1) (Let s e3 e2)) ∧
+  exp_eq_in_ctxt (Bind s e3 c) e1 e2 = exp_eq_in_ctxt c (Let s e3 e1) (Let s e3 e2) ∧
+  exp_eq_in_ctxt (RecBind l c) e1 e2 = exp_eq_in_ctxt c (Letrec l e1) (Letrec l e2)
+End
+
+Definition ctxt_size_def:
+  ctxt_size Nil = 0n ∧
+  ctxt_size (IsFree s ctxt) = 1 + ctxt_size ctxt ∧
+  ctxt_size (Bind s e ctxt) = 1 + list_size char_size s +  exp_size e + ctxt_size ctxt ∧
+  ctxt_size (RecBind sel ctxt) = 1 + exp1_size sel + ctxt_size ctxt
+End
+
+
+Theorem exp_eq_in_ctxt_refl:
+  ∀c e. exp_eq_in_ctxt c e e
+Proof
+  Induct
+  \\ gvs [exp_eq_in_ctxt_def, exp_eq_refl]
+QED
+
+Theorem exp_eq_in_ctxt_sym:
+  ∀c e1 e2. exp_eq_in_ctxt c e1 e2 ⇔ exp_eq_in_ctxt c e2 e1
+Proof
+  Induct
+  \\ rw [] \\ eq_tac
+  \\ gvs [exp_eq_in_ctxt_def, exp_eq_sym]
+QED
+
+Theorem exp_eq_in_ctxt_trans:
+  ∀c e1 e2 e3. exp_eq_in_ctxt c e1 e2 ∧ exp_eq_in_ctxt c e2 e3 ⇒ exp_eq_in_ctxt c e1 e3
+Proof
+  Induct
+  \\ rw []
+  \\ gvs [exp_eq_in_ctxt_def]
+  >- (irule exp_eq_trans
+      \\ pop_assum $ irule_at Any \\ fs [])
+  \\ rw []
+  \\ last_x_assum irule
+  \\ first_x_assum $ irule_at Any
+  \\ gvs []
+QED
+
+Theorem exp_eq_IMP_exp_eq_in_ctxt:
+  ∀c e e'. e ≈ e' ⇒ exp_eq_in_ctxt c e e'
+Proof
+  Induct
+  \\ gvs [exp_eq_in_ctxt_def]
+  \\ rw []
+  \\ first_x_assum irule
+  \\ gvs [exp_eq_Letrec_cong, exp_eq_App_cong, exp_eq_Lam_cong, exp_eq_refl, exp_eq_l_refl]
+QED
+
+Theorem exp_eq_in_ctxt_Prim:
+  ∀c eL eL' ope. LIST_REL (exp_eq_in_ctxt c) eL eL' ⇒ exp_eq_in_ctxt c (Prim ope eL) (Prim ope eL')
+Proof
+  Induct
+  \\ gvs [exp_eq_in_ctxt_def, exp_eq_refl, exp_eq_Prim_cong]
+  \\ rw []
+  \\ irule exp_eq_in_ctxt_trans
+  \\ irule_at Any exp_eq_in_ctxt_trans
+  \\ last_x_assum $ irule_at Any
+  \\ irule_at (Pos last) exp_eq_IMP_exp_eq_in_ctxt
+  \\ irule_at (Pos last) exp_eq_IMP_exp_eq_in_ctxt
+  >~[‘Letrec’]
+  >- (irule_at Any Letrec_Prim
+      \\ irule_at Any $ iffLR exp_eq_sym
+      \\ irule_at Any Letrec_Prim
+      \\ gvs [LIST_REL_EL_EQN, EL_MAP, exp_eq_in_ctxt_def])
+  \\ irule_at Any Let_Prim
+  \\ irule_at Any $ iffLR exp_eq_sym
+  \\ irule_at Any Let_Prim
+  \\ gvs [LIST_REL_EL_EQN, EL_MAP, exp_eq_in_ctxt_def]
+QED
+
+Theorem exp_eq_in_ctxt_App:
+  ∀c f1 f2 e1 e2. exp_eq_in_ctxt c f1 f2 ∧ exp_eq_in_ctxt c e1 e2
+                  ⇒ exp_eq_in_ctxt c (App f1 e1) (App f2 e2)
+Proof
+  Induct
+  \\ gvs [exp_eq_in_ctxt_def,exp_eq_App_cong]
+  \\ rw []
+  \\ irule exp_eq_in_ctxt_trans
+  \\ irule_at Any exp_eq_in_ctxt_trans
+  \\ last_x_assum $ irule_at (Pos $ el 2)
+  \\ first_x_assum $ irule_at (Pos $ el 2)
+  \\ rpt $ last_assum $ irule_at Any
+  \\ gvs [exp_eq_IMP_exp_eq_in_ctxt, Let_App, Letrec_App, exp_eq_sym]
+QED
+
+Theorem exp_eq_in_ctxt_Apps:
+  ∀eL eL' e e' c. LIST_REL (exp_eq_in_ctxt c) eL eL' ⇒ exp_eq_in_ctxt c e e'
+                  ⇒ exp_eq_in_ctxt c (Apps e eL) (Apps e' eL')
+Proof
+  Induct
+  >- (Cases
+      \\ fs [Apps_def])
+  \\ gen_tac
+  \\ Cases
+  \\ rw [Apps_def]
+  \\ first_x_assum irule
+  \\ fs [exp_eq_in_ctxt_App]
+QED
+
+Theorem Let_App_in_ctxt:
+  ∀c s e1 e2 e3. exp_eq_in_ctxt c (Let s e1 (App e2 e3)) (App (Let s e1 e2) (Let s e1 e3))
+Proof
+  rpt gen_tac
+  \\ irule exp_eq_IMP_exp_eq_in_ctxt
+  \\ gvs [Let_App]
+QED
+
+Theorem Let_freevars:
+  ∀c v e e'. v ∉ freevars e' ⇒ exp_eq_in_ctxt c (Let v e e') e'
+Proof
+  rw []
+  \\ irule exp_eq_IMP_exp_eq_in_ctxt
+  \\ irule eval_wh_IMP_exp_eq
+  \\ rw [subst_def, eval_wh_thm, bind1_def, GSYM subst_fdomsub]
+  >- (AP_TERM_TAC
+      \\ irule subst1_ignore
+      \\ rename1 ‘subst f e2’
+      \\ qsuff_tac ‘closed (subst f e2)’
+      >- rw [closed_def]
+      \\ irule IMP_closed_subst
+      \\ rw []
+      \\ first_x_assum $ irule_at Any
+      \\ fs [FRANGE_FLOOKUP]
+      \\ pop_assum $ irule_at Any)
+  \\ gvs [IMP_closed_subst, FRANGE_FLOOKUP]
+QED
+
+Theorem Let_Let_in_ctxt:
+  ∀v w e1 e2 e3 c. v ≠ w ∧ v ∉ freevars e2 ∧ w ∉ freevars e1 ⇒
+                   exp_eq_in_ctxt c (Let v e1 (Let w e2 e3)) (Let w e2 (Let v e1 e3))
+Proof
+  rw []
+  \\ irule exp_eq_IMP_exp_eq_in_ctxt
+  \\ gvs [Let_Let]
+QED
+
+Theorem exp_eq_in_ctxt_Lam:
+  ∀c s e1 e2. exp_eq_in_ctxt (IsFree s c) e1 e2
+              ⇒ exp_eq_in_ctxt c (Lam s e1) (Lam s e2)
+Proof
+  Induct
+  \\ fs[exp_eq_in_ctxt_def] \\ rw [exp_eq_in_ctxt_def]
+  >- (rw [exp_eq_Lam_strong]
+      \\ first_x_assum $ drule_then assume_tac
+      \\ irule exp_eq_trans
+      \\ irule_at Any beta_equality
+      \\ fs []
+      \\ irule $ iffLR exp_eq_sym
+      \\ irule exp_eq_trans
+      \\ irule_at (Pos last) beta_equality
+      \\ fs [exp_eq_sym])
+  >>~ [‘Letrec l (Lam w _)’]
+  >- (‘∃s. s ∉ {w} ∪ set (MAP FST l) ∪ BIGUNION (set (MAP (freevars o SND) l))
+             ∪ freevars e1 ∪ freevars e2’
+        by  (‘INFINITE 𝕌(:string)’ by simp [] \\ dxrule_then assume_tac $ iffLR NOT_IN_FINITE
+             \\ pop_assum $ irule_at Any \\ rw [FINITE_UNION, FINITE_BIGUNION, MEM_EL]
+             \\ gvs [EL_MAP])
+      \\ irule exp_eq_in_ctxt_trans
+      \\ irule_at (Pos hd) exp_eq_IMP_exp_eq_in_ctxt
+      \\ irule_at Any exp_eq_Letrec_cong
+      \\ irule_at Any exp_eq_l_refl
+      \\ irule_at Any exp_alpha_exp_eq
+      \\ irule_at Any exp_alpha_Alpha
+      \\ fs []
+      \\ first_assum $ irule_at Any \\ fs []
+      \\ irule exp_eq_in_ctxt_trans
+      \\ irule_at (Pos hd) exp_eq_IMP_exp_eq_in_ctxt
+      \\ irule_at Any Letrec_Lam_weak
+      \\ conj_tac
+      >- (rw [EVERY_MEM]
+          \\ rename1 ‘MEM e _’ \\ last_x_assum $ qspecl_then [‘freevars e’] assume_tac
+          \\ fs [MEM_MAP]
+          \\ rename1 ‘e = SND pair’ \\ pop_assum $ qspecl_then [‘pair’] assume_tac
+          \\ rw [])
+      \\ fs []
+      \\ irule exp_eq_in_ctxt_trans
+      \\ irule_at (Pos last) exp_eq_IMP_exp_eq_in_ctxt
+      \\ irule_at Any $ iffLR exp_eq_sym
+      \\ irule_at Any exp_eq_Letrec_cong
+      \\ irule_at Any exp_alpha_exp_eq
+      \\ irule_at Any exp_alpha_Alpha
+      \\ irule_at Any exp_eq_l_refl
+      \\ first_assum $ irule_at Any \\ fs []
+      \\ irule exp_eq_in_ctxt_trans
+      \\ irule_at (Pos last) exp_eq_IMP_exp_eq_in_ctxt
+      \\ irule_at Any $ iffLR exp_eq_sym
+      \\ irule_at Any Letrec_Lam_weak
+      \\ fs []
+      \\ conj_tac
+      >- (rw [EVERY_MEM]
+          \\ rename1 ‘MEM e _’ \\ last_x_assum $ qspecl_then [‘freevars e’] assume_tac
+          \\ fs [MEM_MAP]
+          \\ rename1 ‘e = SND pair’ \\ pop_assum $ qspecl_then [‘pair’] assume_tac
+          \\ rw [])
+      \\ last_x_assum irule
+      \\ rw []
+      \\ irule exp_eq_in_ctxt_trans
+      \\ irule_at Any exp_eq_in_ctxt_trans
+      \\ last_x_assum $ irule_at Any
+      \\ first_assum $ irule_at Any
+      \\ irule_at (Pos last) $ iffLR exp_eq_in_ctxt_sym
+      \\ conj_tac
+      \\ irule exp_eq_IMP_exp_eq_in_ctxt
+      \\ irule exp_eq_trans
+      \\ irule_at Any Let_Letrec
+      \\ fs []
+      \\ irule_at Any exp_eq_Letrec_cong
+      \\ irule_at Any $ iffLR exp_eq_sym
+      \\ irule_at Any exp_eq_App_cong
+      \\ irule_at Any exp_alpha_exp_eq
+      \\ irule_at Any exp_alpha_Alpha
+      \\ rw [EVERY_MEM, exp_eq_refl, exp_eq_l_refl]
+      \\ rename1 ‘MEM e _’
+      \\ last_x_assum $ qspecl_then [‘freevars e’] assume_tac
+      \\ fs [MEM_MAP]
+      \\ rename1 ‘e = SND pair’ \\ pop_assum $ qspecl_then [‘pair’] assume_tac
+      \\ rw [])
+  \\ rename1 ‘Let v e3 (Lam w _)’
+  \\ ‘∃s. s ∉ {v} ∪ {w} ∪ freevars e3 ∪ freevars e1 ∪ freevars e2’
+    by (‘INFINITE 𝕌(:string)’ by simp []
+        \\ gvs [NOT_IN_FINITE])
+  \\ irule exp_eq_in_ctxt_trans
+  \\ irule_at (Pos hd) exp_eq_IMP_exp_eq_in_ctxt
+  \\ irule_at Any exp_eq_App_cong \\ irule_at Any exp_eq_Lam_cong
+  \\ irule_at Any exp_alpha_exp_eq
+  \\ irule_at Any exp_alpha_Alpha
+  \\ fs [] \\ first_assum $ irule_at Any
+  \\ irule_at Any exp_eq_refl \\ fs []
+  \\ irule exp_eq_in_ctxt_trans
+  \\ irule_at (Pos hd) exp_eq_IMP_exp_eq_in_ctxt
+  \\ irule_at Any Let_Lam_weak \\ fs []
+  \\ irule exp_eq_in_ctxt_trans
+  \\ irule_at (Pos last) exp_eq_IMP_exp_eq_in_ctxt
+  \\ irule_at Any $ iffLR exp_eq_sym
+  \\ irule_at Any exp_eq_App_cong \\ irule_at Any exp_eq_Lam_cong
+  \\ irule_at Any exp_alpha_exp_eq
+  \\ irule_at Any exp_alpha_Alpha
+  \\ first_assum $ irule_at Any
+  \\ irule_at Any exp_eq_refl \\ fs []
+  \\ irule exp_eq_in_ctxt_trans
+  \\ irule_at (Pos last) exp_eq_IMP_exp_eq_in_ctxt
+  \\ irule_at Any $ iffLR exp_eq_sym
+  \\ irule_at Any Let_Lam_weak \\ fs []
+  \\ last_x_assum $ irule_at Any
+  \\ rw []
+  \\ irule exp_eq_in_ctxt_trans \\ irule_at Any exp_eq_in_ctxt_trans
+  \\ last_x_assum $ irule_at Any
+  \\ first_assum $ irule_at (Pos hd)
+  \\ rpt $ irule_at Any exp_eq_IMP_exp_eq_in_ctxt
+  \\ TRY $ last_assum $ irule_at Any
+  \\ irule_at (Pos last) $ iffLR exp_eq_sym
+  \\ conj_tac
+  \\ irule exp_eq_trans
+  \\ irule_at (Pos last) Let_Let
+  \\ gvs [closed_def]
+  \\ irule exp_eq_App_cong \\ fs [exp_eq_refl]
+  \\ irule exp_eq_Lam_cong
+  \\ irule exp_eq_App_cong \\ fs [exp_eq_refl]
+  \\ irule exp_alpha_exp_eq
+  \\ irule exp_alpha_Alpha
+  \\ fs []
+QED
+
+Theorem exp_eq_in_ctxt_Lams:
+  ∀vl c e e'. exp_eq_in_ctxt (FOLDL (λc n. IsFree n c) c vl) e e' ⇒
+              exp_eq_in_ctxt c (Lams vl e) (Lams vl e')
+Proof
+  Induct
+  \\ rw [Lams_def]
+  \\ irule exp_eq_in_ctxt_Lam
+  \\ last_x_assum $ irule_at Any
+  \\ fs []
+QED
+
+val _ = export_theory();
